more

Weidenbach_Book/Watched_Literals_Watch_List.thy
@@ -287,7 +287,7 @@ definition blits_in_\<L>\<^sub>i\<^sub>n :: \<open>'v twl_st_wl \<Rightarrow> bo
   \<open>blits_in_\<L>\<^sub>i\<^sub>n S == (\<forall>L \<in># all_lits_st S. \<forall>(i, K, b) \<in> set (watched_by S L). K \<in># all_lits_st S)\<close>
 
 
-definition literals_are_\<L>\<^sub>i\<^sub>n :: \<open>nat multiset \<Rightarrow> nat twl_st_wl \<Rightarrow> bool\<close> where
+definition literals_are_\<L>\<^sub>i\<^sub>n :: \<open>'v multiset \<Rightarrow> 'v twl_st_wl \<Rightarrow> bool\<close> where
   \<open>literals_are_\<L>\<^sub>i\<^sub>n \<A> S \<equiv> (is_\<L>\<^sub>a\<^sub>l\<^sub>l \<A> (all_lits_st S) \<and> blits_in_\<L>\<^sub>i\<^sub>n S)\<close>
 
 
